Switch pure_semantics to use new eval_wh

language/pure_semanticsScript.sml
@@ -5,6 +5,9 @@ open arithmeticTheory listTheory stringTheory alistTheory optionTheory
 
 val _ = new_theory "pure_semantics";
 
+
+(* definitions *)
+
 Datatype:
   result = SilentDivergence
          | Termination
@@ -12,39 +15,48 @@ Datatype:
 End
 
 Datatype:
-  next_res = Act 'e (v list) | Ret | Div | Err
+  next_res = Act 'e (exp list) | Ret | Div | Err
 End
 
 Inductive next:
-  (∀e stack.
-    next (Constructor "Act" [e], stack) (Act e stack))
+  (∀e stack a.
+    eval_wh e = wh_Atom a ⇒
+    next (wh_Constructor "Act" [e], stack) (Act a stack))
   ∧
   (∀m f stack res.
-    next (m, f::stack) res ⇒
-    next (Constructor "Bind" [m; f], stack) res)
+    next (eval_wh m, f::stack) res ⇒
+    next (wh_Constructor "Bind" [m; f], stack) res)
   ∧
   (∀stack.
-    next (Diverge, stack) Div)
+    next (wh_Diverge, stack) Div)
   ∧
   (∀v.
-    next (Constructor "Ret" [v], []) Ret)
+    next (wh_Constructor "Ret" [v], []) Ret)
   ∧
-  (∀v f n e x stack res.
-    dest_Closure f = SOME (n,e) ∧ eval x = v ∧
-    next (eval (bind n x e), stack) res ⇒
-    next (Constructor "Ret" [v], f::stack) res)
+  (∀f n e x stack res.
+    dest_wh_Closure (eval_wh f) = SOME (n,e) ∧
+    next (eval_wh (bind n x e), stack) res ⇒
+    next (wh_Constructor "Ret" [x], f::stack) res)
+  ∧
+  (∀f x stack.
+    eval_wh f = wh_Diverge ⇒
+    next (wh_Constructor "Ret" [x], f::stack) Div)
   ∧
   (∀v stack.
-    (v ≠ Diverge) ∧
-    (∃e. v ≠ Constructor "Act" [e]) ∧
-    (∃e. v ≠ Constructor "Ret" [e]) ∧
-    (∃m f. v ≠ Constructor "Bind" [m; f]) ⇒
+    (v ≠ wh_Diverge) ∧
+    (∀e. v = wh_Constructor "Act" [e] ⇒
+         ∀a. eval_wh e ≠ wh_Atom a) ∧
+    (∀e. v = wh_Constructor "Ret" [e] ⇒
+         stack ≠ [] ∧
+         ∀f fs. stack = f :: fs ⇒ eval_wh f ≠ wh_Diverge ∧
+                                  dest_wh_Closure (eval_wh f) = NONE) ∧
+    (∀m f. v ≠ wh_Constructor "Bind" [m; f]) ⇒
     next (v, stack) Err)
 End
 
 Definition next_action_def:
-  next_action (v, stack) =
-    case some res. next (v, stack) res of
+  next_action (wh, stack) =
+    case some res. next (wh, stack) res of
     | SOME res => res
     | NONE => Div
 End
@@ -52,56 +64,121 @@ End
 Definition continue_def:
   continue [] k = INL T ∧
   continue (f::stack) k =
-    case dest_Closure f of
+    case dest_wh_Closure (eval_wh f) of
     | NONE => INL F
-    | SOME (n,e) => INR (eval (bind n (Lit k) e), stack)
+    | SOME (n,e) => INR (eval_wh (bind n (Lit k) e), stack)
 End
 
 Definition interp'_def:
   interp' =
     io_unfold
-      (λi. case i of
-           | INL T => Ret' Termination
-           | INL F => Ret' Error
-           | INR (v, stack) =>
-             case next_action (v,stack) of
-             | Ret => Ret' Termination
-             | Err => Ret' Error
-             | Div => Ret' SilentDivergence
-             | Act a new_stack => Vis' a (continue new_stack))
+      (λ(v,stack). case next_action (v,stack) of
+                   | Ret => Ret' Termination
+                   | Err => Ret' Error
+                   | Div => Ret' SilentDivergence
+                   | Act a new_stack =>
+                       Vis' a (λy. (wh_Constructor "Ret" [Lit y], new_stack)))
 End
 
 Definition interp_def:
-  interp v stack = interp' (INR (v, stack))
+  interp v stack = interp' (v, stack)
 End
 
 Theorem interp_def:
-  interp v stack =
-    case next_action (v,stack) of
+  interp wh stack =
+    case next_action (wh,stack) of
     | Ret => Ret Termination
     | Div => Ret SilentDivergence
     | Err => Ret Error
     | Act a new_stack =>
-        Vis a (λk. case continue new_stack k of
-                   | INL b => Ret (if b then Termination else Error)
-                   | INR (v,stack) => interp v stack)
+        Vis a (λy. interp (wh_Constructor "Ret" [Lit y]) new_stack)
 Proof
   fs [Once interp_def,interp'_def]
   \\ once_rewrite_tac [io_unfold] \\ fs []
-  \\ Cases_on ‘next_action (v,stack)’ \\ fs []
+  \\ Cases_on ‘next_action (wh,stack)’ \\ fs []
   \\ fs [combinTheory.o_DEF,FUN_EQ_THM] \\ rw []
-  \\ Cases_on ‘continue l k’ \\ fs []
-  THEN1
-   (once_rewrite_tac [io_unfold] \\ fs []
-    \\ IF_CASES_TAC \\ fs [])
-  \\ CASE_TAC \\ fs []
-  \\ fs [Once interp_def,interp'_def]
+  \\ once_rewrite_tac [EQ_SYM_EQ]
+  \\ fs [interp_def,interp'_def]
+  \\ simp [Once io_unfold] \\ fs []
 QED
 
 Definition semantics_def:
-  semantics e binds = interp (eval e) (MAP eval binds)
+  semantics e binds = interp (eval_wh e) binds
 End
 
-(* TODO: derive nice equations for reasoning about semantics *)
+
+(* descriptive lemmas *)
+
+Overload Ret = “λx. Cons "Ret" [x]”
+Overload Act = “λx. Cons "Act" [x]”
+Overload Bind = “λx y. Cons "Bind" [x;y]”
+
+Theorem semanitcs_Ret:
+  semantics (Ret x) [] = Ret Termination
+Proof
+  fs [semantics_def,eval_wh_Cons]
+  \\ simp [Once interp_def]
+  \\ fs [next_action_def]
+  \\ simp [Once next_cases]
+QED
+
+Theorem semanitcs_Ret_App:
+  semantics (Ret x) (f::fs) = semantics (App f x) fs
+Proof
+  fs [semantics_def,eval_wh_Cons]
+  \\ simp [Once interp_def]
+  \\ fs [next_action_def]
+  \\ simp [Once next_cases]
+  \\ Cases_on ‘dest_wh_Closure (eval_wh f)’ \\ fs []
+  THEN1
+    (fs [eval_wh_thm]
+     \\ Cases_on ‘eval_wh f = wh_Diverge’ \\ fs []
+     \\ simp [Once interp_def]
+     \\ fs [next_action_def]
+     \\ simp [Once next_cases])
+  \\ rename [‘_ = SOME xx’] \\ PairCases_on ‘xx’ \\ fs []
+  \\ fs [eval_wh_thm]
+  \\ Cases_on ‘eval_wh f = wh_Diverge’ \\ fs []
+  \\ once_rewrite_tac [EQ_SYM_EQ]
+  \\ simp [Once interp_def]
+  \\ fs [next_action_def]
+QED
+
+Theorem semanitcs_Bottom:
+  semantics Bottom xs = Ret SilentDivergence
+Proof
+  fs [semantics_def,eval_wh_Bottom]
+  \\ simp [Once interp_def]
+  \\ fs [next_action_def]
+  \\ simp [Once next_cases]
+QED
+
+Theorem semanitcs_Bind:
+  semantics (Bind x f) fs = semantics x (f::fs)
+Proof
+  fs [semantics_def,eval_wh_Cons]
+  \\ simp [Once interp_def]
+  \\ fs [next_action_def]
+  \\ simp [Once next_cases]
+  \\ once_rewrite_tac [EQ_SYM_EQ]
+  \\ simp [Once interp_def]
+  \\ fs [next_action_def]
+QED
+
+Theorem semanitcs_Act:
+  semantics (Act x) fs =
+    case eval x of
+    | Atom a => Vis a (λy. semantics (Ret (Lit y)) fs)
+    | _      => Ret Error
+Proof
+  fs [semantics_def,eval_wh_Cons]
+  \\ simp [Once interp_def]
+  \\ fs [next_action_def]
+  \\ simp [Once next_cases,eval_wh_Lit]
+  \\ Cases_on ‘∃a. eval_wh x = wh_Atom a’ \\ fs []
+  \\ fs [eval_def,Once v_unfold]
+  \\ Cases_on ‘eval_wh x’ \\ fs []
+QED
+
 
 val _ = export_theory();
